new commit

Automata/Common.lean
@@ -30,12 +30,13 @@ def falseDFA: DFA (Fin 0) (Fin 1) := {
 
 def eqBase (k: ℕ) : DFA (Fin 2 → Fin k) (Fin 2) := {
   transition := fun f s => match s with
-    | 0 => if (f 0).val == f 1 then 0 else 1
+    | 0 => if (f 0).val = f 1 then 0 else 1
     | 1 => 1
   start := 0
   output := fun x => x == 0
 }
 
+#eval (eqBase 2).eval (inputToBase 2 (by norm_num) [2, 2])
 --Exists x, x = 0?
 #eval (project (eqBase 2) (by norm_num) ⟨0, by norm_num⟩).eval [fun _ => 0]
 
@@ -47,14 +48,24 @@ def eqBase' (k: ℕ) (a b n : ℕ) (ha: a < n) (hb: b < n): DFA (Fin n → Fin k
   output := fun x => x == 0
 }
 
-#eval (eqBase 2).eval [fun _ => 0, fun _ => 1]
-#eval (eqBase 2).eval [fun x => x, fun x => x]
 #eval (eqBase' 2 0 1 2 (by norm_num) (by norm_num)).eval [fun _ => 0, fun _ => 1]
 #eval (eqBase' 2 0 1 2 (by norm_num) (by norm_num)).eval [fun x => x, fun x => x]
 
+
+def leBase (k: ℕ)  : DFA (Fin 2 → Fin k) (Fin 2) := {
+  transition := fun f s => match s with
+    | 0 => if (f 0).val <= (f 1).val then 0 else 1
+    | 1 => 1
+  start := 0
+  output := fun x => x == 0
+}
+
+-- Exists x, not 0 <= x?
+#eval (project ((leBase 2).negate) (by norm_num) ⟨1, by norm_num⟩).eval [fun _ => 0]
+
 def addBase (k: ℕ) : DFA (Fin 3 → Fin k) (Fin 3) := {
   transition := fun f s => match s with
-    | 0 => if f 0 + f 1 == f 2 then 0 else
+    | 0 => if (f 0).val + f 1 == f 2 then 0 else
       if (f 0).val + f 1 + 1 == f 2 then 1
       else 2
     | 1 => if (f 0).val + f 1 + 1 == f 2 + k then 1 else
@@ -65,52 +76,118 @@ def addBase (k: ℕ) : DFA (Fin 3 → Fin k) (Fin 3) := {
   output := fun x => x == 0
 }
 
-def ltBase (k: ℕ)  : DFA (Fin 2 → Fin k) (Fin 3) := {
-  transition := fun f s => match s with
-    | 0 => if (f 0).val < (f 1).val then 1 else if (f 0).val == (f 1).val then 0 else 2
-    | 1 => 1
-    | 2 => 2
-  start := 0
-  output := fun x => x == 1
-}
-
--- Exists x, x < 0?
-#eval (project (ltBase 2) (by norm_num) ⟨0, by norm_num⟩).eval [fun _ => 0]
-
---Exists x, x + 1 = 0? Wrong Answer!
+--Exists x, x + 1 = 0?
 #eval (project (addBase 2) (by norm_num) ⟨0, by norm_num⟩).evalFrom [fun x => if x == 0 then 1 else 0] [0]
+--Exists x, 1 + 1 = x?
+#eval (project (addBase 2) (by norm_num) ⟨2, by norm_num⟩).evalFrom [fun _ => 1] [0]
 
+--FIX: Exists x, 1 + 1 = x?
+#eval (project (addBase 2) (by norm_num) ⟨2, by norm_num⟩).evalFrom [fun _ => 0, fun _ => 1] [0]
 
+/- Try to prove eqBase is correct
 
-theorem eqBase_if_equal_aux (b : ℕ) (m n : ℕ) (hb: b > 1):
-  m = n → (eqBase b).evalFrom (inputToBase b hb [m, n]) 0 := by
+1. DFA accepts iff f 0 = f 1 for all f ∈ input
+2. input natural numbers are equal iff f 0 = f 1 for all f ∈ input
+
+-/
+theorem eqBase_if_equal_aux (b : ℕ) (input: List (Fin 2 → Fin b)):
+  (∀ f ∈ input, (f 0).val = f 1) → (eqBase b).evalFrom input 0 := by
   intro h
-  rw[h]
-  generalize hl: (inputToBase b hb [n, n]).length = l
-  induction l with
-  | zero =>
-    simp only [List.length_eq_zero] at hl
-    rw[hl]
-    simp[eqBase, DFAO.evalFrom]
-  | succ l ih =>
+  induction input
+  case nil =>
+    simp[eqBase, DFAO.evalFrom, DFAO.transFrom]
+  case cons f fs ih =>
+    have h1 := h f
+    simp only [List.mem_cons, true_or, Fin.isValue, true_implies] at h1
+    simp only [DFAO.evalFrom, DFAO.transFrom, Fin.isValue]
+    have: ((eqBase b).transition f 0) = 0 := by
+      simp only [eqBase, Fin.isValue, beq_iff_eq, h1, ↓reduceIte]
+    rw[this]
+    apply ih
+    intro f' hf'
+    apply h
+    simp only [List.mem_cons, or_true, hf']
+
+example (k : ℕ) (state : Fin 2) (f : Fin 2 → Fin k) :
+  (eqBase k).transition f state = 0 →  state = 0 ∧ (f 0).val = f 1 := by
+  simp[eqBase, DFAO.transition]
+  split <;> simp
+
+theorem eqBase_trans_zero (k : ℕ) (state : Fin 2) (f : Fin 2 → Fin k) :
+  (eqBase k).transition f state = 0 ↔ state = 0 ∧ (f 0).val == f 1 := by
+  constructor
+  intro h1
+  simp[eqBase] at h1
+  constructor
+  . by_contra h
+    have: state = 1 := by exact Fin.eq_one_of_neq_zero state h
+    simp[this] at h1
+  . simp only [Fin.isValue, beq_iff_eq]
+    have: ¬state = 0 → state = 1 := by intro hns; exact Fin.eq_one_of_neq_zero state hns
+    have: state = 0 ∨ state = 1 := by tauto
+    rcases this with hs | hs
+    . simp only [hs, Fin.isValue, ite_eq_then, one_ne_zero, imp_false, Decidable.not_not] at h1
+      exact h1
+    . simp only [hs, Fin.isValue, one_ne_zero] at h1
+  intro h
+  rcases h with ⟨h1, h2⟩
+  simp only [Fin.isValue, beq_iff_eq] at h2
+  simp only [eqBase, Fin.isValue, beq_iff_eq, ↓reduceIte, h1, h2]
+
+theorem eqBase_transFrom_zero (k : ℕ) (state: Fin 2) (l : List (Fin 2 → Fin k)) :
+  (eqBase k).transFrom l state = 0 ↔ state = 0 ∧ ∀ f ∈ l, (f 0).val = f 1 := by
+  induction l generalizing state
+  case nil =>
+    simp[eqBase, DFAO.transFrom]
+  case cons f fs ih =>
+    simp[DFAO.transFrom]
+    specialize ih ((eqBase k).transition f state)
+    constructor
+    . intro h
+      have:= ih.mp h
+      rcases this with ⟨h1, h2⟩
+      have:= (eqBase_trans_zero k state f).mp h1
+      rcases this with ⟨h3, h4⟩
+      constructor
+      . exact h3
+      . constructor
+        . simp only [Fin.isValue, beq_iff_eq] at h4
+          exact h4
+        . exact h2
+    . intro h
+      rcases h with ⟨h1, h2, h3⟩
+      apply ih.mpr
+      constructor
+      . apply (eqBase_trans_zero k state f).mpr
+        constructor
+        . exact h1
+        . simp only [Fin.isValue, beq_iff_eq]
+          exact h2
+      . exact h3
+
+theorem equal_if_eqBase_aux_aux (b : ℕ) (input: List (Fin 2 → Fin b)):
+  (eqBase b).transFrom input 0 = 0 → (∀ f ∈ input, (f 0).val = f 1) := by
+  intro h
+  exact (eqBase_transFrom_zero b 0 input).mp h |>.2
+  -- exact this.2
+
+theorem equal_if_eqBase_aux (b : ℕ) (input: List (Fin 2 → Fin b)):
+  (eqBase b).evalFrom input 0 → (∀ f ∈ input, (f 0).val = f 1) := by
+  intro h
+  have:= equal_if_eqBase_aux_aux b input
+  apply this
+  simp[DFAO.evalFrom, DFAO.output, eqBase] at h
+  apply h
 
 
-  sorry
+
+
+
+
+
 
 
 
 theorem eqBase_if_equal (b : ℕ) (m n : ℕ) (hb: b > 1):
   m = n → (eqBase b).eval (inputToBase b hb [m, n]) := by
-  rw[DFAO.eval]
-  intro h
-  rw[h]
-  generalize hl: (inputToBase b hb [n, n]).length = l
-  induction l with
-  | zero =>
-    simp only [List.length_eq_zero] at hl
-    rw[hl]
-    simp[eqBase, DFAO.evalFrom]
-  | succ l ih =>
-
-
   sorry
